

## Gross entropy

$$E = - \sum_i [t_i \log(y_i) + (1-t_i) \log(1-y_i)]$$

$$\frac{\partial E}{\partial y_i} = - \left[ \frac{t_i}{y_i} + (1-t_i)(-1) \left( \frac{1}{1-y_i} \right) \right]$$

$$= \frac{1-t_i}{1-y_i} - \frac{t_i}{y_i}$$

$$\frac{\partial y_i}{\partial s_i} = y_i \cdot (1-y_i)$$

$$\delta = y_i \cdot (1-y_i) \cdot \left[ \frac{1-t_i}{1-y_i} - \frac{t_i}{y_i} \right]$$

$$= \left[ y_i \cdot (1-t_i) - t_i \cdot (1-y_i) \right]$$

$$= y_i - \cancel{y_i t_i} - t_i + \cancel{y_i t_i}$$